skip_list/inv/skip_inv.v
@@ -17,80 +17,93 @@ Module SkipListInv (Params: SKIP_LIST_PARAMS).
   Export Invariant.
 
   Section Proofs.
-    Context `{!heapGS Σ, !gset_list_unionGS Σ, lockG Σ} (N : namespace).
+    Context `{!heapGS Σ, !gset_list_unionGS Σ, !lockG Σ}.
 
     Definition levelN (lvl: Z) := nroot .@ "level" .@ lvl.
 
-    Definition from_sub_list (bot: gset node_rep) (curr: node_rep) : iProp Σ := 
+    Definition from_sub_list (bot: lazy_gname) (curr: node_rep) : iProp Σ := 
       ∃ (l: loc) (down: node_rep),
       ⌜ node_down curr = Some l ⌝
       ∗
       l ↦ rep_to_node down
       ∗
-      ⌜ down ∈ bot ⌝
+      own (s_auth bot) (◯ {[ down ]})
       ∗
       ⌜ node_key curr = node_key down ⌝.
 
     Definition from_bot_list (curr: node_rep) : iProp Σ := 
       ⌜ node_down curr = None ⌝.
 
-    Fixpoint skip_list_equiv (head: node_rep) (lvl: Z) (L: list (gset node_rep)) (S: gset node_rep) : iProp Σ :=
+    Fixpoint skip_list_equiv (head: node_rep) (lvl: Z) (L: list lazy_gname) : iProp Σ :=
       match L with
       | nil => False
       | top :: bots =>
         match bots with
-        | nil => ⌜ lvl = 0 ⌝
-                 ∗
-                 inv (levelN lvl) (lazy_list_inv head top from_bot_list)
-                 ∗
-                 ⌜ node_down head = None ⌝
-                 ∗
-                 ⌜ top = S ⌝
+        | nil => 
+          ⌜ lvl = 1 ⌝
+          ∗
+          inv (levelN lvl) (lazy_list_inv head top from_bot_list)
+          ∗
+          ⌜ node_down head = None ⌝
                  
-        | bot :: _ => ∃ (l: loc) (down: node_rep),
-                      ⌜ lvl > 0 ⌝
-                      ∗
-                      inv (levelN lvl) (lazy_list_inv head top (from_sub_list bot))
-                      ∗
-                      ⌜ node_down head = Some l ⌝
-                      ∗
-                      l ↦ rep_to_node down
-                      ∗
-                      ⌜ node_key head = node_key down ⌝
-                      ∗
-                      skip_list_equiv down (lvl - 1) bots S
+        | bot :: _ => 
+          ∃ (l: loc) (down: node_rep),
+            ⌜ lvl > 1 ⌝
+            ∗
+            inv (levelN lvl) (lazy_list_inv head top (from_sub_list bot))
+            ∗
+            ⌜ node_down head = Some l ⌝
+            ∗
+            l ↦ rep_to_node down
+            ∗
+            ⌜ node_key head = node_key down ⌝
+            ∗
+            skip_list_equiv down (lvl - 1) bots
         end
       end.
 
-    Definition is_skip_list (v: val) (Skeys: gset Z) : iProp Σ := 
-      ∃ (l:loc) (head: node_rep) (S: gset node_rep) (L: list (gset node_rep)),
-      ⌜ key_equiv S Skeys ⌝
-      ∗
+    Fixpoint own_frac (q: frac) (L_gset: list (gset Z)) (L_gname: list lazy_gname) : iProp Σ :=
+      match L_gset, L_gname with
+      | nil, nil => True
+      | Stop :: Sbots, top :: bots =>
+        ∃ (Sfrac: gset node_rep),
+          ⌜ key_equiv Sfrac Stop ⌝
+          ∗
+          own (s_frac top) (◯F{q} Sfrac)
+          ∗
+          own_frac q Sbots bots
+      | _, _ => False
+      end.
+
+    Definition is_skip_list (v: val) (q: frac) (L_gset: list (gset Z)) (L_gname: list lazy_gname) : iProp Σ := 
+      ∃ (l:loc) (head: node_rep),
       ⌜ #l = v ⌝
       ∗
       l ↦ rep_to_node head
       ∗
       ⌜ node_key head = INT_MIN ⌝
       ∗
-      skip_list_equiv head MAX_HEIGHT L S.
+      own_frac q L_gset L_gname
+      ∗
+      skip_list_equiv head MAX_HEIGHT L_gname.
 
 
-    Lemma skip_list_equiv_cons_inv (top_head: node_rep) (lvl: Z) (S: gset node_rep)
-      (L: list (gset node_rep)) (top: gset node_rep) :
-      skip_list_equiv top_head lvl (top :: L) S ⊢ 
+    Lemma skip_list_equiv_cons_inv (top_head: node_rep) (lvl: Z)
+      (top: lazy_gname) (bots: list lazy_gname) :
+      skip_list_equiv top_head lvl (top :: bots) ⊢ 
         ∃ (P: node_rep → iProp Σ),
         inv (levelN lvl) (lazy_list_inv top_head top P)
         ∗
-        skip_list_equiv top_head lvl (top :: L) S
+        skip_list_equiv top_head lvl (top :: bots)
     .
     Proof.
-      destruct L as [|bot].
+      destruct bots as [|bot].
       + iIntros "Htop". iExists from_bot_list.
-        iDestruct "Htop" as "(%Hlvl & #Hinv & %Hnone & %Heq)".
-        by iFrame "#".
+        iDestruct "Htop" as "(? & #? & ?)".
+        iFrame "# ∗".
       + iIntros "Hlist". iExists (from_sub_list bot).
-        iDestruct "Hlist" as (l down) "(%Hlvl & #Hinv & %Hsome & Hpt & Hmatch)".
-        iFrame "#". iExists l, down. by iFrame.
+        iDestruct "Hlist" as (l down) "(? & #? & ? & ? & ?)".
+        iFrame "# ∗". iExists l, down. iFrame "# ∗".
     Qed.
 
   End Proofs.
