skip_list/spec/new.v
@@ -3,7 +3,7 @@ From iris.heap_lang Require Import proofmode.
 
 From SkipList.lib Require Import lock misc.
 From SkipList.skip_list Require Import node_rep code key_equiv.
-From SkipList.skip_list.inv Require Import skip_inv.
+From SkipList.skip_list.inv Require Import lazy_inv skip_inv.
 
 
 Local Open Scope Z.
@@ -13,105 +13,169 @@ Module NewSpec (Params: SKIP_LIST_PARAMS).
   Import Invariant.
 
   Section Proofs.
-    Context `{!heapGS Σ, !gset_list_unionGS Σ, lockG Σ} (N : namespace).
+    Context `{!heapGS Σ, !gset_list_unionGS Σ, !lockG Σ}.
 
-    Theorem newLoop_spec (head: node_rep) (lvl: Z) (L: list (gset node_rep)):
+    Fixpoint is_empty (L: list (gset Z)) (lvl: Z) : iProp Σ :=
+      match L with
+      | nil => ⌜ lvl = 0 ⌝
+      | h :: t => ⌜ h = ∅ ⌝
+                  ∗
+                  is_empty t (lvl - 1)
+      end.
+
+    Theorem newLoop_spec (head: node_rep) (lvl: Z) (Sbots: list (gset Z))
+      (bot: lazy_gname) (bots: list lazy_gname) :
       {{{ 
         ⌜ node_key head = INT_MIN ⌝
         ∗
-        ⌜ 0 ≤ lvl ⌝
+        ⌜ 1 ≤ lvl ⌝
         ∗
-        skip_list_equiv head lvl (∅ :: L) ∅ 
+        is_empty (∅ :: Sbots) lvl
+        ∗
+        own_frac 1 (∅ :: Sbots) (bot :: bots)
+        ∗
+        skip_list_equiv head lvl (bot :: bots)
       }}}
         newLoop (rep_to_node head) #lvl
-      {{{ h top_head L', RET #h;
+      {{{ h top_head L_gset L_gname, RET #h;
         h ↦ rep_to_node top_head
         ∗
         ⌜ node_key top_head = INT_MIN ⌝
         ∗
-        skip_list_equiv top_head MAX_HEIGHT L' ∅ 
+        is_empty L_gset MAX_HEIGHT
+        ∗
+        own_frac 1 L_gset L_gname
+        ∗
+        skip_list_equiv top_head MAX_HEIGHT L_gname
       }}}.
     Proof.
-      iIntros (Φ) "(Hmin & Hlvl & Hlist) HΦ".
-      iRevert (head lvl L) "Hmin Hlvl Hlist HΦ".
+      iIntros (Φ) "(Hmin & Hlvl & Hempty & Hown & Hlist) HΦ".
+      iRevert (head lvl Sbots bot bots) "Hmin Hlvl Hempty Hown Hlist HΦ".
       iLöb as "IH".
-      iIntros (head lvl L) "%Hmin %Hlvl Hlist HΦ".
+      iIntros (head lvl Sbots bot bots) "%Hmin %Hlvl Hempty Hown Hlist HΦ".
 
       wp_lam. wp_let. wp_alloc h as "Hh".
       wp_pures. case_bool_decide; wp_if.
       + iApply "HΦ". iModIntro.
         assert (lvl = MAX_HEIGHT) as <- by congruence.
         by iFrame.
-      + wp_alloc t as "Ht". wp_let.
+      + iMod (own_alloc (● (∅ : gset node_rep) ⋅ ◯ (∅: gset node_rep)))
+          as (γauth) "[Hown_auth Hown_auth_frag]"; 
+          first by apply auth_both_valid.
+        iMod (own_alloc (●F (∅ : gset node_rep) ⋅ ◯F (∅: gset node_rep)))
+          as (γfrac) "[Hown_frac Hown_frac_frag]"; 
+          first by apply auth_both_valid.
+        iMod (own_alloc (GSet (Zlt_range INT_MIN INT_MAX)))
+          as (γtok) "Hown_tok"; first done.
+
+        assert (GSet (Zlt_range INT_MIN INT_MAX) =
+          GSet (Zlt_range INT_MIN INT_MAX) ⋅ GSet (∅)) as ->.
+        { rewrite gset_disj_union; f_equal; set_solver. }
+        iDestruct "Hown_tok" as "(Hown_tok & Hown_emp)".
+      
+        wp_alloc t as "Ht". wp_let.
         iDestruct "Ht" as "(Ht1 & Ht2)".
-        wp_apply (newlock_spec (node_inv t) with "[Ht1]").
+        wp_apply (newlock_spec (node_inv t γtok (INT_MIN)) with "[Ht1 Hown_tok]").
         { iExists tail; iFrame. }
+        
         iIntros (l) "#Hlock". iDestruct "Hlock" as (γ) "Hlock".
         wp_pures.
         set (top_head := (INT_MIN, Some t, Some h, l)).
         rewrite (fold_rep_to_node top_head).
 
-        iMod (inv_alloc (levelN (lvl + 1)) ⊤ (lazy_list_inv top_head ∅ (from_sub_list ∅)) 
-          with "[Ht2]") as "#Hinv".
+        set (Γ := mk_lazy_gname γauth γfrac γtok).
+        iMod (inv_alloc (levelN (lvl + 1)) ⊤ (lazy_list_inv top_head Γ (from_sub_list ∅)) 
+          with "[Ht2 Hlock Hown_auth Hown_frac Hown_emp]") as "#Hinv".
         {
-          iNext. iExists nil.
+          iNext. iExists ∅, ∅, nil. iFrame.
           iSplit; first done. iSplit.
           {
             assert (node_lt top_head tail); last (simpl; auto).
             rewrite /node_lt/node_key//=; apply HMIN_MAX.
           }
+          iSplit; first rewrite /key_equiv //.
           iExists t, γ. by iFrame "# ∗".
         }
 
-        iApply ("IH" $! top_head (lvl+1) (∅ :: L) with "[%] [%] [Hlist Hh]").
+        iApply ("IH" $! top_head (lvl+1) (∅ :: Sbots) Γ (bot :: bots) 
+          with "[%] [%] [Hempty] [Hown Hown_frac_frag] [Hlist Hh]").
         { done. }
         { lia. }
         { 
+          rewrite /is_empty.
+          assert (lvl + 1 - 1 = lvl) as -> by lia.
+          by iFrame.
+        }
+        { iExists ∅; iFrame. rewrite /key_equiv //. }
+        {
           iExists h, head.
           assert (lvl + 1 - 1 = lvl) as -> by lia.
-          iSplit; first by iPureIntro; lia.
-          by iFrame "# ∗".
+          iFrame "# ∗". iPureIntro.
+          by split; first lia.
         }
         
-        iNext; iApply "HΦ".
+        iNext. iApply "HΦ".
     Qed.
 
     Theorem new_spec : 
       {{{ True }}}
         new #()
-      {{{ v, RET v;
-        is_skip_list v ∅
+      {{{ v S L, RET v;
+        is_skip_list v 1 S L
+        ∗
+        is_empty S MAX_HEIGHT
       }}}.
     Proof.
       iIntros (Φ) "_ HΦ".
+
+      iMod (own_alloc (● (∅ : gset node_rep) ⋅ ◯ (∅: gset node_rep)))
+        as (γauth) "[Hown_auth Hown_auth_frag]"; 
+        first by apply auth_both_valid.
+      iMod (own_alloc (●F (∅ : gset node_rep) ⋅ ◯F (∅: gset node_rep)))
+        as (γfrac) "[Hown_frac Hown_frac_frag]"; 
+        first by apply auth_both_valid.
+      iMod (own_alloc (GSet (Zlt_range INT_MIN INT_MAX)))
+        as (γtok) "Hown_tok"; first done.
+
+      assert (GSet (Zlt_range INT_MIN INT_MAX) =
+        GSet (Zlt_range INT_MIN INT_MAX) ⋅ GSet (∅)) as ->.
+      { rewrite gset_disj_union; f_equal; set_solver. }
+      iDestruct "Hown_tok" as "(Hown_tok & Hown_emp)".
+
       wp_lam. wp_alloc t as "Ht". wp_let.
       iDestruct "Ht" as "(Ht1 & Ht2)".
-      wp_apply (newlock_spec (node_inv t) with "[Ht1]").
+      wp_apply (newlock_spec (node_inv t γtok (INT_MIN)) with "[Ht1 Hown_tok]").
       { iExists tail; iFrame. }
+
       iIntros (l) "#Hlock". iDestruct "Hlock" as (γ) "Hlock".
       wp_pures.
       rewrite (fold_rep_to_node (INT_MIN, Some t, None, l)).
       set (bot_head := (INT_MIN, Some t, None, l)).
 
-      iMod (inv_alloc (levelN 0) ⊤ (lazy_list_inv bot_head ∅ from_bot_list) 
-        with "[Ht2]") as "#Hbot_inv".
+      set (Γ := mk_lazy_gname γauth γfrac γtok).
+      iMod (inv_alloc (levelN 1) ⊤ (lazy_list_inv bot_head Γ from_bot_list) 
+        with "[Ht2 Hlock Hown_auth Hown_frac Hown_emp]") as "#Hinv".
       {
-        iNext. iExists nil.
+        iNext. iExists ∅, ∅, nil. iFrame.
         iSplit; first done. iSplit.
         {
           assert (node_lt bot_head tail); last (simpl; auto).
           rewrite /node_lt/node_key//=; apply HMIN_MAX.
         }
+        iSplit; first rewrite /key_equiv //.
         iExists t, γ. by iFrame "# ∗".
       }
 
-      wp_apply (newLoop_spec _ _ nil).
-      { by iFrame "# ∗". }
+      wp_apply (newLoop_spec _ _ nil Γ nil with "[Hown_frac_frag]").
+      {
+        iSplit; first done. iSplit; first done. iSplit; first done.
+        iSplit. iExists ∅; iFrame. rewrite /key_equiv //.
+        by iFrame "# ∗".
+      }
 
-      iIntros (h top_head L) "(Hh & %Hmin & Hlist)"; wp_let.
-      iModIntro; iApply "HΦ". 
-      iExists h, top_head, ∅, L.
-      iSplit; first rewrite /key_equiv //.
+      iIntros (h top_head S L) "(Hh & %Hmin & Hempty & Hlist)"; wp_let.
+      iModIntro; iApply "HΦ".
+      iFrame "# ∗". iExists h, top_head.
       by iFrame.
     Qed.
 
