skip_list/spec/contains.v
@@ -5,6 +5,7 @@ From iris.heap_lang Require Import proofmode.
 
 From SkipList.lib Require Import lock misc.
 From SkipList.skip_list Require Import node_rep code key_equiv.
+From SkipList.skip_list.inv Require Import lazy_inv skip_inv.
 From SkipList.skip_list.spec Require Import find.
 
 
@@ -15,43 +16,63 @@ Module ContainsSpec (Params: SKIP_LIST_PARAMS).
   Import Find.
 
   Section Proofs.
-    Context `{!heapGS Σ, !gset_list_unionGS Σ, lockG Σ} (N : namespace).
+    Context `{!heapGS Σ, !gset_list_unionGS Σ, !lockG Σ}.
     
-    Theorem findPred_spec (curr top_head: node_rep) (top: gset node_rep) 
-      (lvl: Z) (key: Z) (L: list (gset node_rep)) (S: gset node_rep) :
+    Theorem findPred_spec (curr top_head: node_rep) (lvl: Z) (key: Z)
+      (Sfrac: gset node_rep) (Stop: gset Z) (Sbots: list (gset Z)) 
+      (top: lazy_gname) (bots: list lazy_gname) :
       {{{ 
-        skip_list_equiv top_head lvl (top :: L) S
+        skip_list_equiv top_head lvl (top :: bots)
         ∗
-        ⌜ curr = top_head ∨ curr ∈ top ⌝
+        own_frac 1 Sbots bots
+        ∗
+        own (s_frac top) (◯F Sfrac)
+        ∗
+        ⌜ key_equiv Sfrac Stop ⌝
+        ∗
+        (⌜ curr = top_head ⌝ ∨ own (s_auth top) (◯ {[curr]}))
         ∗
         ⌜ node_key curr < key < INT_MAX ⌝
       }}}
         findPred (rep_to_node curr) #key
-      {{{ pred succ, RET SOMEV ((rep_to_node pred), (rep_to_node succ));
-        skip_list_equiv top_head lvl (top :: L) S
+      {{{ pred succ S, RET SOMEV ((rep_to_node pred), (rep_to_node succ));
+        skip_list_equiv top_head lvl (top :: bots)
         ∗
-        ⌜ key ∈ map node_key (elements S) ↔ node_key succ = key ⌝
+        own_frac 1 (Stop :: Sbots) (top :: bots)
+        ∗
+        ⌜ last (Stop :: Sbots) = Some S ⌝
+        ∗
+        ⌜ key ∈ S ↔ node_key succ = key ⌝
       }}}.
     Proof.
-      iIntros (Φ) "(Hlist & Hcurr_range & Hrange) HΦ".
-      iRevert (curr lvl top_head top L) "Hlist Hcurr_range Hrange HΦ".
+      iIntros (Φ) "(Hlist & Hown & Hown_frag & Hequiv & Hcurr_range & Hrange) HΦ".
+      iRevert (curr top_head lvl Sfrac Stop Sbots top bots) "Hlist Hown Hown_frag Hequiv Hcurr_range Hrange HΦ".
       iLöb as "IH".
-      iIntros (curr lvl top_head top L) "Hlist %Hcurr_range %Hrange HΦ".
-
-      iPoseProof (skip_list_equiv_cons_inv top_head lvl S L top with "Hlist") as "Hlist".
-      iDestruct "Hlist" as (P) "(Hinv & Hlist)".
+      iIntros (curr top_head lvl Sfrac Stop Sbots top bots) "Hlist Hown Hown_frag %Hequiv #Hcurr_range %Hrange HΦ".
 
       wp_lam. wp_let.
-      wp_apply (find_spec with "[Hinv]").
-      { by iFrame. }
+      iPoseProof (skip_list_equiv_cons_inv with "Hlist") as "Hlist".
+      iDestruct "Hlist" as (P) "(Hinv & Hlist)".
+      wp_apply (find_spec with "[Hinv Hown_frag]").
+      { by iFrame "# ∗". }
 
-      iIntros (pred succ) "(%Hpred_range & %Hpred_key & %Hkey_in_S)".
+      iIntros (pred succ) "(Hown_frag & %Hpred_range & %Hpred_key & %Hkey_in_S)".
       wp_pures. wp_lam. wp_pures.
       destruct (node_down pred) as [d|] eqn:Hcurr_down; wp_pures.
       + wp_bind (Load _).
-        destruct L as [|bot].
-        - iDestruct "Hlist" as "(%Hlvl & #Hinv & %Hnone & Heq)".
-          iInv (levelN lvl) as (L') "(>%Hperm & >%Hsort & Hlist)" "Hclose".
+        destruct bots as [|bot].
+        - iDestruct "Hlist" as "(%Hlvl & #Hinv & %Hnone)".
+          iInv (levelN lvl) as (S Skeys L) "(>%Hperm & >%Hsort & >%Hequiv' & Hown_auth & Hown_frac & Hown_tok & Hlist)" "Hclose".
+          iMod "Hown_frac"; iDestruct (own_valid_2 with "Hown_frac Hown_frag") 
+            as %<-%frac_auth_agree_L.
+          
+          iMod "Hown_auth"; iAssert ((⌜ curr = top_head ∨ curr ∈ S ⌝)%I) with "[Hown_auth Hcurr_range]" as %Hcurr_range.
+          {
+            iDestruct "Hcurr_range" as "[Heq|Hown]"; first by iLeft.
+            iDestruct (own_valid_2 with "Hown_auth Hown") 
+              as %[Hvalid%gset_included]%auth_both_valid_discrete.
+            iPureIntro; right; set_solver.
+          }
 
           destruct Hpred_range as [|Hin]; first by congruence.
           rewrite -elem_of_elements elem_of_list_In -Hperm in Hin.
@@ -59,54 +80,68 @@ Module ContainsSpec (Params: SKIP_LIST_PARAMS).
           iDestruct "Hlist" as (? ? ?) "(_ & _ & _ & _ & HP & _)".
           iMod "HP" as %Hfalse; congruence.
         - iDestruct "Hlist" as (l down) "(%Hlvl & #Hinv & %Hsome & Hpt & %Hmin & Hmatch)".
-          iInv (levelN lvl) as (L') "(>%Hperm & >%Hsort & Hlist)" "Hclose".
+          iInv (levelN lvl) as (S Skeys L) "(>%Hperm & >%Hsort & >%Hequiv' & Hown_auth & Hown_frac & Hown_tok & Hlist)" "Hclose".
+          iMod "Hown_frac"; iDestruct (own_valid_2 with "Hown_frac Hown_frag") 
+            as %<-%frac_auth_agree_L.
+
+          destruct Sbots as [|Sbot]; first by iExFalso.
+          iDestruct "Hown" as (Sbot_frag) "(? & ? & ?)".
 
           destruct Hpred_range as [Heq|Hin].
           * assert (d = l) as -> by congruence.
             wp_load.
-            iMod ("Hclose" with "[Hlist]") as "_".
-            { iNext; iExists L'; by iFrame. }
+            iMod ("Hclose" with "[Hlist Hown_auth Hown_frac Hown_tok]") as "_".
+            { iNext; iExists S, Skeys, L; by iFrame. }
 
             iModIntro; wp_let.
-            iApply ("IH" $! down (lvl - 1) down bot L with "[$] [%] [%]").
-            { by left. }
+            iApply ("IH" with "[$] [$] [$] [$] [] [%]").
+            { by iLeft. }
             { rewrite -Hmin -Heq; lia. }
-            iNext; iIntros (pred' succ') "(Hlist & %Hkey_in_S')".
-            iApply "HΦ"; iSplit; last done. 
-            iExists l, down. by iFrame "# ∗".
+            iNext; iIntros (pred' succ' Sfrac') "(Hlist & Hown & %Hlast & %Hkey_in_S')".
+            iApply "HΦ". 
+            iSplitL "Hpt Hlist". iExists l, down. by iFrame "# ∗".
+            iSplitL "Hown Hown_frag". iExists S. by iFrame.
+            done.
           * rewrite -elem_of_elements elem_of_list_In -Hperm in Hin.
             rewrite list_equiv_invert_L; last done.
             iDestruct "Hlist" as (succ' l' γ) "(Hsucc'_range & Hsome' & Hpt' & Hlock & HP & Himp)".
-            iDestruct "HP" as (d' down') "(Hsome_down & Hpt_down & Hin_bot & Hdown'_key)".
-            iMod "Hsome_down" as %Hsome_down; 
-            iMod "Hin_bot" as %Hin_bot; 
+            iDestruct "HP" as (d' down') "(Hsome_down & Hpt_down & Hown_down' & Hdown'_key)".
+            iMod "Hsome_down" as %Hsome_down;
             iMod "Hdown'_key" as %Hdown'_key.
-            
+
+            iMod "Hown_down'".
+            assert ({[down']} ≡ {[down']} ⋅ {[down']}) as -> by set_solver.
+            iDestruct "Hown_down'" as "(Hown_down' & Hown_down'_dup)".
+
             assert (d = d') as <- by congruence.
             iMod "Hpt_down"; wp_load.
-            iMod ("Hclose" with "[Hpt' Hpt_down Himp]") as "_".
-            { 
-              iNext; iExists L'.
-              iPoseProof ("Himp" with "[Hpt' Hpt_down]") as "Hlist".
-              { iFrame; iExists d, down'; by iFrame. }
-              by iFrame.
-            }
+            iPoseProof ("Himp" with "[Hpt' Hpt_down Hown_down']") as "Hlist".
+            { iFrame; iExists d, down'; by iFrame. }
+            iMod ("Hclose" with "[Hown_auth Hown_frac Hown_tok Hlist]") as "_".
+            { iNext; iExists S, Skeys, L. by iFrame. }
 
             iModIntro; wp_let.
             iDestruct "Hsucc'_range" as %Hsucc'_range; 
             iDestruct "Hsome'" as %Hsome'.
-            iApply ("IH" $! down' (lvl - 1) down bot L with "[$] [%] [%]").
-            { by right. }
+            iApply ("IH" with "[$] [$] [$] [$] [Hown_down'_dup] [%]").
+            { by iRight. }
             { rewrite -Hdown'_key; lia. }
-            iNext; iIntros (pred'' succ'') "(Hlist & %Hkey_in_S'')".
-            iApply "HΦ"; iSplit; last done.
-            iExists l, down. by iFrame "# ∗".
-      + destruct L as [|bot].
+            iNext; iIntros (pred'' succ'' S'') "(Hlist & Hown & %Hlast & %Hkey_in_S'')".
+            iApply "HΦ".
+            iSplitL "Hpt Hlist". iExists l, down. by iFrame "# ∗".
+            iSplitL "Hown Hown_frag". iExists S. by iFrame.
+            done.
+      + destruct bots as [|bot].
         - iModIntro. iApply "HΦ".
-          iDestruct "Hlist" as "(%Hlvl & #Hinv & %Hnone & %Heq)".
-          rewrite -Heq; by iFrame "#".
-        - iDestruct "Hlist" as (l down) "(%Hlvl & #Hinv & %Hsome & Hpt & Hmatch)".
-          iInv (levelN lvl) as (L') "(>%Hperm & >%Hsort & Hlist)" "Hclose".
+          iDestruct "Hlist" as "(%Hlvl & #Hinv & %Hnone)".
+          iSplit. by iFrame "#".
+          iSplit. iExists Sfrac. by iFrame.
+          iSplit; last by rewrite -Hequiv elem_of_elements in Hkey_in_S.
+          by destruct Sbots; last by iExFalso.
+        - iDestruct "Hlist" as (l down) "(%Hlvl & #Hinv & %Hsome & Hpt & %Heq & Hmatch)".
+          iInv (levelN lvl) as (S Skeys L) "(>%Hperm & >%Hsort & >%Hequiv' & Hown_auth & Hown_frac & Hown_tok & Hlist)" "Hclose".
+          iMod "Hown_frac"; iDestruct (own_valid_2 with "Hown_frac Hown_frag") 
+            as %<-%frac_auth_agree_L.
 
           destruct Hpred_range as [|Hin]; first by congruence.
           rewrite -elem_of_elements elem_of_list_In -Hperm in Hin.
@@ -116,38 +151,39 @@ Module ContainsSpec (Params: SKIP_LIST_PARAMS).
           iMod "Hfalse" as %Hfalse; congruence.
     Qed.
     
-    Theorem contains_spec (v: val) (key: Z) (Skeys: gset Z)
+    Theorem contains_spec (v: val) (key: Z) 
+      (L_gset: list (gset Z)) (L_gname: list lazy_gname)
       (Hrange: INT_MIN < key < INT_MAX) :
-      {{{ is_skip_list v Skeys }}}
+      {{{ is_skip_list v 1 L_gset L_gname }}}
         contains v #key
-      {{{ (b: bool), RET #b; 
-        is_skip_list v Skeys
+      {{{ (b: bool) S, RET #b; 
+        is_skip_list v 1 L_gset L_gname
         ∗
-        ⌜ if b then key ∈ Skeys else key ∉ Skeys ⌝
+        ⌜ last L_gset = Some S ⌝
+        ∗
+        ⌜ if b then key ∈ S else key ∉ S ⌝
       }}}.
     Proof.
       iIntros (Φ) "H HΦ".
-      iDestruct "H" as (h head S L) "(%Hequiv & %Hv & Hpt & %Hmin & Hlist)".
+      iDestruct "H" as (h head) "(%Hv & Hpt & %Hmin & Hown_frac & Hlist)".
       wp_lam. wp_let. rewrite -Hv. wp_load.
-      destruct L as [|l L]; first by iExFalso.
-      wp_apply (findPred_spec with "[Hlist]").
-      { iFrame "# ∗". iPureIntro; split. by left. lia. }
-      iIntros (pred succ) "(Hlist & %Hkey_in_S)".
-      wp_let. wp_match. wp_pures. wp_lam. wp_pures.
+      destruct L_gname as [|top bots]; destruct L_gset as [|Stop Sbots]; try by iExFalso.
+      iDestruct "Hown_frac" as (Sfrac) "(Hequiv & Hown & Hown_frac)".
+      wp_apply (findPred_spec with "[Hlist Hequiv Hown Hown_frac]").
+      { iFrame. iSplit. by iLeft. iPureIntro; lia. }
 
+      iIntros (pred succ S) "(Hlist & Hown_frac & %Hlast & %Hkey_in_S)".
+      wp_let. wp_match. wp_pures. wp_lam. wp_pures.
       iModIntro; case_bool_decide.
+      + iApply "HΦ". iSplit.
+        { iExists h, head. by iFrame. }
+        iPureIntro; split; first done.
+        rewrite Hkey_in_S; congruence.
       + iApply "HΦ". iSplit. 
-        iExists h, head, S, (l :: L).
-        { by iFrame "# ∗". }
-        iPureIntro. rewrite /key_equiv in Hequiv. 
-        rewrite -elem_of_elements Hequiv Hkey_in_S.
-        congruence.
-      + iApply "HΦ". iSplit. 
-        iExists h, head, S, (l :: L).
-        { by iFrame "# ∗". }
-        iPureIntro. intros Hin. 
-        rewrite -elem_of_elements Hequiv Hkey_in_S in Hin.
-        congruence.
+        { iExists h, head. by iFrame. }
+        iPureIntro; split; first done.
+        intros Hin. 
+        rewrite Hkey_in_S in Hin; congruence.
     Qed.
 
   End Proofs.
